examples/blocks_dom.pddl
@@ -1,0 +1,45 @@
+;;;;;;;;;;;;;;;;;;;;;;;;;;;;;;;;;;;;;;;;
+;;; 4 Op-blocks world
+;;;;;;;;;;;;;;;;;;;;;;;;;;;;;;;;;;;;;;;;
+
+(define (domain BlocksDom)
+  (:requirements :strips :negative-preconditions :equality :disjunctive-preconditions)
+  (:predicates (on ?x ?y)
+	       (ontable ?x)
+	       (handempty)
+	       (holding ?x)
+         )
+
+  (:action pick-up
+	     :parameters (?x)
+	     :precondition (and (forall (?z) (not (on ?z ?x))) (ontable ?x) (handempty))
+	     :effect
+	     (and (not (ontable ?x))
+		   (not (handempty))
+		   (holding ?x)))
+
+  (:action put-down
+	     :parameters (?x)
+	     :precondition (holding ?x)
+	     :effect
+	     (and (not (holding ?x))
+		   (handempty)
+		   (ontable ?x)))
+
+  (:action stack
+	     :parameters (?x ?y)
+	     :precondition (and (holding ?x) (forall (?z ?a) (or (not (= ?a ?y)) (not (on ?z ?a)))))
+	     :effect
+	     (and (not (holding ?x))
+		   (handempty)
+		   (on ?x ?y)))
+
+  (:action unstack
+	     :parameters (?x ?y)
+	     :precondition (and (on ?x ?y) (not (exists (?z) (on ?z ?x))) (handempty))
+	     :effect
+	     (and (holding ?x)
+		   (not (handempty))
+		   (not (on ?x ?y))))
+)
+
